proof/theories/Payload_Break.v
@@ -46,7 +46,7 @@ Definition bad_pkt : packet :=
      pkt_xfrm := fun _ _ _ => []; pkt_ctdir := fun _ _ => [];
      pkt_inner := fun _ _ _ _ => [];
      pkt_have_l4 := false;     (* NFT_PKTINFO_L4PROTO not set -> transport read BREAKs *)
-     pkt_fragoff := 0; pkt_flow := []; pkt_untracked := false |}.
+     pkt_fragoff := 0; pkt_flow := []; pkt_untracked := false; pkt_ctdir_orig := true |}.
 
 (** The transport read fails (the kernel would NFT_BREAK). *)
 Lemma bad_pkt_th_breaks : read_payload_ok PTransport 2 2 bad_pkt = false.
@@ -105,7 +105,7 @@ Definition frag_pkt : packet :=
      pkt_xfrm := fun _ _ _ => []; pkt_ctdir := fun _ _ => [];
      pkt_inner := fun _ _ _ _ => [];
      pkt_have_l4 := true;
-     pkt_fragoff := 8; pkt_flow := []; pkt_untracked := false |}.   (* a non-first fragment *)
+     pkt_fragoff := 8; pkt_flow := []; pkt_untracked := false; pkt_ctdir_orig := true |}.   (* a non-first fragment *)
 
 Theorem neq_dport_frag_no_match :
   eval_matchcond (MNeq FThDport [0; 22]) frag_pkt = false.
